Prove reorder rel-fence; instr

src/trans/ReorderRelFence.v
@@ -22,6 +22,7 @@ Require Import Thread.
 Require Import Configuration.
 
 Require Import Progress.
+Require Import ReorderInternal.
 
 Require Import SimLocal.
 Require Import SimMemory.
@@ -29,16 +30,13 @@ Require Import SimGlobal.
 Require Import SimThread.
 Require Import Compatibility.
 
-Require Import ReorderStep.
-Require Import ReorderRelFenceCommon.
-
 Require Import ITreeLang.
 Require Import ITreeLib.
 
 Set Implicit Arguments.
 
 
-Inductive reorder_release_fenceF: forall R (i2:MemE.t R), Prop :=
+Variant reorder_release_fenceF: forall R (i2:MemE.t R), Prop :=
 | reorder_release_fenceF_load
     l2 o2:
     reorder_release_fenceF (MemE.read l2 o2)
@@ -55,79 +53,399 @@ Inductive reorder_release_fenceF: forall R (i2:MemE.t R), Prop :=
     reorder_release_fenceF (MemE.fence Ordering.acqrel Ordering.plain)
 .
 
-Inductive sim_release_fenceF: forall R
-                                     (st_src:itree MemE.t (unit * R)%type) (lc_src:Local.t) (sc1_src:TimeMap.t) (mem1_src:Memory.t)
-                                     (st_tgt:itree MemE.t (unit * R)%type) (lc_tgt:Local.t) (sc1_tgt:TimeMap.t) (mem1_tgt:Memory.t), Prop :=
+Definition local_relfenced (lc:Local.t) :=
+  (Local.mk (TView.mk
+               (fun _ => (TView.cur (Local.tview lc)))
+               (TView.cur (Local.tview lc))
+               (TView.acq (Local.tview lc)))
+            (Local.promises lc)
+            (Local.reserves lc)).
+
+Lemma local_relfenced_wf
+      lc gl
+      (WF: Local.wf lc gl):
+  Local.wf (local_relfenced lc) gl.
+Proof.
+  inv WF. econs; ss; eauto.
+  - inv TVIEW_WF. econs; ss. refl.
+  - inv TVIEW_CLOSED. econs; ss.
+Qed.
+
+Lemma local_relfenced_sim_local
+      lc gl
+      (WF: Local.wf lc gl):
+  sim_local lc (local_relfenced lc).
+Proof.
+  econs; ss. econs; try refl; apply WF.
+Qed.
+
+Lemma sim_local_relfenced
+      lc_src
+      lc_tgt gl_tgt
+      (LOCAL: sim_local lc_src lc_tgt)
+      (LC_WF_TGT: Local.wf lc_tgt gl_tgt):
+  sim_local lc_src (local_relfenced lc_tgt).
+Proof.
+  etrans; eauto using local_relfenced_sim_local.
+Qed.
+
+Lemma sim_local_internal_relfenced
+      e
+      lc1_src gl1_src
+      lc1_tgt gl1_tgt
+      lc2_tgt gl2_tgt
+      (STEP_TGT: Local.internal_step e lc1_tgt gl1_tgt lc2_tgt gl2_tgt)
+      (LOCAL1: sim_local lc1_src (local_relfenced lc1_tgt))
+      (GLOBAL1: sim_global gl1_src gl1_tgt)
+      (LC_WF1_SRC: Local.wf lc1_src gl1_src)
+      (LC_WF1_TGT: Local.wf lc1_tgt gl1_tgt)
+      (GL_WF1_SRC: Global.wf gl1_src)
+      (GL_WF1_TGT: Global.wf gl1_tgt):
+  exists lc2_src gl2_src,
+    <<STEP_SRC: Local.internal_step e lc1_src gl1_src lc2_src gl2_src>> /\
+    <<LOCAL2: sim_local lc2_src (local_relfenced lc2_tgt)>> /\
+    <<GLOBAL2: sim_global gl2_src gl2_tgt>>.
+Proof.
+  exploit local_relfenced_wf; try exact LC_WF1_TGT. i.
+  exploit sim_local_internal; try exact LOCAL1; eauto.
+  unfold local_relfenced. destruct lc1_tgt.
+  inv STEP_TGT; inv LOCAL; ss; eauto.
+Qed.
+
+Lemma sim_local_read_relfenced
+      lc1_src gl1_src
+      lc1_tgt gl1_tgt
+      lc2_tgt
+      loc ts val released_tgt ord_src ord_tgt
+      (STEP_TGT: Local.read_step lc1_tgt gl1_tgt loc ts val released_tgt ord_tgt lc2_tgt)
+      (LOCAL1: sim_local lc1_src (local_relfenced lc1_tgt))
+      (GLOBAL1: sim_global gl1_src gl1_tgt)
+      (LC_WF1_SRC: Local.wf lc1_src gl1_src)
+      (LC_WF1_TGT: Local.wf lc1_tgt gl1_tgt)
+      (GL_WF1_SRC: Global.wf gl1_src)
+      (GL_WF1_TGT: Global.wf gl1_tgt)
+      (ORD: Ordering.le ord_src ord_tgt):
+  exists released_src lc2_src,
+    <<REL: View.opt_le released_src released_tgt>> /\
+    <<STEP_SRC: Local.read_step lc1_src gl1_src loc ts val released_src ord_src lc2_src>> /\
+    <<LOCAL2: sim_local lc2_src (local_relfenced lc2_tgt)>>.
+Proof.
+  inv LOCAL1. inv STEP_TGT.
+  exploit sim_memory_get; try exact GET; try apply GLOBAL1. i. des. inv MSG.
+  esplits; eauto.
+  - econs; eauto; try by etrans; eauto.
+    eapply TViewFacts.readable_mon; eauto. apply TVIEW.
+  - econs; eauto. inv TVIEW. ss. econs; s.
+    + i. unfold LocFun.find. etrans; [apply LC_WF1_SRC|].
+      eauto using View.join_l.
+    + repeat apply View.join_le; ss.
+      * unfold View.singleton_ur_if. repeat condtac; viewtac.
+      * repeat condtac; viewtac.
+    + repeat apply View.join_le; ss.
+      * unfold View.singleton_ur_if. repeat condtac; viewtac.
+      * repeat condtac; viewtac.
+Qed.
+
+Lemma sim_local_write_relfenced
+      lc1_src gl1_src
+      lc1_tgt gl1_tgt
+      lc2_tgt gl2_tgt
+      loc from to val releasedm_src releasedm_tgt released_tgt ord_src ord_tgt
+      (RELM_LE: View.opt_le releasedm_src releasedm_tgt)
+      (RELM_WF_SRC: View.opt_wf releasedm_src)
+      (RELM_CLOSED_SRC: Memory.closed_opt_view releasedm_src (Global.memory gl1_src))
+      (RELM_WF_TGT: View.opt_wf releasedm_tgt)
+      (ORD_TGT: Ordering.le ord_tgt Ordering.plain \/ Ordering.le Ordering.acqrel ord_tgt)
+      (ORD: Ordering.le ord_src ord_tgt)
+      (STEP_TGT: Local.write_step lc1_tgt gl1_tgt loc from to val releasedm_tgt released_tgt ord_tgt lc2_tgt gl2_tgt)
+      (LOCAL1: sim_local lc1_src (local_relfenced lc1_tgt))
+      (GLOBAL1: sim_global gl1_src gl1_tgt)
+      (LC_WF1_SRC: Local.wf lc1_src gl1_src)
+      (LC_WF1_TGT: Local.wf lc1_tgt gl1_tgt)
+      (GL_WF1_SRC: Global.wf gl1_src)
+      (GL_WF1_TGT: Global.wf gl1_tgt):
+  exists released_src lc2_src gl2_src,
+    <<STEP_SRC: Local.write_step lc1_src gl1_src loc from to val releasedm_src released_src ord_src lc2_src gl2_src>> /\
+    <<RELEASED: View.opt_le released_src released_tgt>> /\
+    <<LOCAL2: sim_local lc2_src (local_relfenced lc2_tgt)>> /\
+    <<GLOBAL2: sim_global gl2_src gl2_tgt>>.
+Proof.
+  guardH ORD_TGT. inv STEP_TGT.
+  assert (REL:
+   View.opt_le
+     (TView.write_released (Local.tview lc1_src) loc to releasedm_src ord_src)
+     (TView.write_released (Local.tview lc1_tgt) loc to releasedm_tgt ord_tgt)).
+  { unfold TView.write_released.
+    condtac; [|econs].
+    condtac; try by (destruct ord_src, ord_tgt; ss).
+    econs. unfold TView.write_tview. s.
+    repeat (condtac; aggrtac); try by apply LC_WF1_TGT.
+    + rewrite <- View.join_r. rewrite <- ? View.join_l. apply LOCAL1.
+    + rewrite <- View.join_r. rewrite <- ? View.join_l.
+      etrans; [|apply LOCAL1]. apply LC_WF1_SRC.
+    + unguard. des; destruct ord_src, ord_tgt; ss.
+  }
+  assert (REL_WF:
+   View.opt_wf (TView.write_released (Local.tview lc1_src) loc to releasedm_src ord_src)).
+  { unfold TView.write_released. condtac; econs.
+    repeat (try condtac; viewtac; try apply LC_WF1_SRC).
+  }
+  exploit sim_memory_add_exists; try exact WRITE; try apply GLOBAL1.
+  { econs 1. exact REL_WF. }
+  { econs; try exact REL; try refl.
+    apply ord_implb. eassumption.
+  }
+  i. des.
+  exploit sim_local_fulfill; try apply LOCAL1; eauto. i.
+  esplits.
+  - econs; eauto.
+    eapply TViewFacts.writable_mon; try exact WRITABLE; eauto. apply LOCAL1.
+  - ss.
+  - inv LOCAL1. ss. econs; ss. inv TVIEW. econs; ss.
+    + i. rewrite LocFun.add_spec. condtac; ss.
+      * subst. unfold LocFun.find.
+        condtac; apply View.join_le; viewtac.
+        etrans; eauto. refl.
+      * unfold LocFun.find. etrans; [apply LC_WF1_SRC|].
+        eauto using View.join_l.
+    + apply View.join_le; viewtac.
+    + apply View.join_le; viewtac.
+  - econs; ss. apply GLOBAL1.
+Qed.
+
+Lemma sim_local_update_relfenced
+      lc1_src gl1_src
+      lc1_tgt gl1_tgt
+      lc2_tgt
+      lc3_tgt gl3_tgt
+      loc ts1 val1 released1_tgt ord1_src ord1_tgt
+      from2 to2 val2 released2_tgt ord2_src ord2_tgt
+      (STEP1_TGT: Local.read_step lc1_tgt gl1_tgt loc ts1 val1 released1_tgt ord1_tgt lc2_tgt)
+      (STEP2_TGT: Local.write_step lc2_tgt gl1_tgt loc from2 to2 val2 released1_tgt released2_tgt ord2_tgt lc3_tgt gl3_tgt)
+      (LOCAL1: sim_local lc1_src (local_relfenced lc1_tgt))
+      (GLOBAL1: sim_global gl1_src gl1_tgt)
+      (LC_WF1_SRC: Local.wf lc1_src gl1_src)
+      (LC_WF1_TGT: Local.wf lc1_tgt gl1_tgt)
+      (GL_WF1_SRC: Global.wf gl1_src)
+      (GL_WF1_TGT: Global.wf gl1_tgt)
+      (ORD1: Ordering.le ord1_src ord1_tgt)
+      (ORD2: Ordering.le ord2_src ord2_tgt)
+      (ORD2_TGT: Ordering.le ord2_tgt Ordering.plain \/ Ordering.le Ordering.acqrel ord2_tgt):
+  exists released1_src released2_src lc2_src lc3_src gl3_src,
+    <<REL1: View.opt_le released1_src released1_tgt>> /\
+    <<REL2: View.opt_le released2_src released2_tgt>> /\
+    <<STEP1_SRC: Local.read_step lc1_src gl1_src loc ts1 val1 released1_src ord1_src lc2_src>> /\
+    <<STEP2_SRC: Local.write_step lc2_src gl1_src loc from2 to2 val2 released1_src released2_src ord2_src lc3_src gl3_src>> /\
+    <<LOCAL3: sim_local lc3_src (local_relfenced lc3_tgt)>> /\
+    <<GLOBAL3: sim_global gl3_src gl3_tgt>>.
+Proof.
+  guardH ORD2_TGT.
+  exploit Local.read_step_future; eauto. i. des.
+  exploit sim_local_read_relfenced; eauto. i. des.
+  exploit Local.read_step_future; eauto. i. des.
+  hexploit sim_local_write_relfenced; eauto. i. des.
+  esplits; eauto.
+Qed.
+
+Lemma sim_local_fence_relfenced
+      lc1_src gl1_src
+      lc1_tgt gl1_tgt
+      lc2_tgt gl2_tgt
+      ordr_src ordw_src
+      ordr_tgt ordw_tgt
+      (STEP_TGT: Local.fence_step lc1_tgt gl1_tgt ordr_tgt ordw_tgt lc2_tgt gl2_tgt)
+      (LOCAL1: sim_local lc1_src (local_relfenced lc1_tgt))
+      (GLOBAL1: sim_global gl1_src gl1_tgt)
+      (LC_WF1_SRC: Local.wf lc1_src gl1_src)
+      (LC_WF1_TGT: Local.wf lc1_tgt gl1_tgt)
+      (ORDR: Ordering.le ordr_src ordr_tgt)
+      (ORDW: Ordering.le ordw_src ordw_tgt)
+      (ORDR_TGT: Ordering.le ordr_tgt Ordering.acqrel)
+      (ORDW_TGT: Ordering.le ordw_tgt Ordering.relaxed):
+  exists lc2_src gl2_src,
+    <<STEP_SRC: Local.fence_step lc1_src gl1_src ordr_src ordw_src lc2_src gl2_src>> /\
+    <<LOCAL2: sim_local lc2_src (local_relfenced lc2_tgt)>> /\
+    <<GLOBAL2: sim_global gl2_src gl2_tgt>>.
+Proof.
+  inv STEP_TGT. esplits.
+  - econs; eauto.
+    i. inv LOCAL1. ss. rewrite PROMISES0.
+    apply PROMISES. destruct ordw_src, ordw_tgt; ss.
+  - inv LOCAL1. inv TVIEW. econs; ss.
+    econs; s; unfold LocFun.find; repeat condtac; aggrtac.
+    + etrans; eauto. apply LC_WF1_TGT.
+    + etrans; eauto. apply LC_WF1_TGT.
+    + etrans; eauto. apply LC_WF1_TGT.
+  - inv GLOBAL1. econs; ss.
+    unfold TView.write_fence_sc.
+    repeat (condtac; viewtac).
+Qed.
+
+Lemma sim_local_is_racy_relfenced
+      lc1_src gl1_src
+      lc1_tgt gl1_tgt
+      loc to ord_src ord_tgt
+      (STEP_TGT: Local.is_racy lc1_tgt gl1_tgt loc to ord_tgt)
+      (LOCAL1: sim_local lc1_src (local_relfenced lc1_tgt))
+      (GLOBAL1: sim_global gl1_src gl1_tgt)
+      (ORD: Ordering.le ord_src ord_tgt):
+  <<STEP_SRC: Local.is_racy lc1_src gl1_src loc to ord_src>>.
+Proof.
+  inv LOCAL1. inv GLOBAL1. inv STEP_TGT; ss.
+  - econs; congr.
+  - exploit sim_memory_get; try exact GET; try eassumption. i. des. inv MSG0.
+    econs; try exact GET0.
+    + eapply TViewFacts.racy_view_mon; eauto. apply TVIEW.
+    + i. destruct na, na1; ss.
+      exploit MSG; ss. destruct ord_src, ord_tgt; ss.
+Qed.
+
+Lemma sim_local_racy_read_relfenced
+      lc1_src gl1_src
+      lc1_tgt gl1_tgt
+      loc to val ord_src ord_tgt
+      (STEP_TGT: Local.racy_read_step lc1_tgt gl1_tgt loc to val ord_tgt)
+      (LOCAL1: sim_local lc1_src (local_relfenced lc1_tgt))
+      (GLOBAL1: sim_global gl1_src gl1_tgt)
+      (ORD: Ordering.le ord_src ord_tgt):
+  <<STEP_SRC: Local.racy_read_step lc1_src gl1_src loc to val ord_src>>.
+Proof.
+  inv STEP_TGT.
+  exploit sim_local_is_racy_relfenced; eauto.
+Qed.
+
+Lemma sim_local_racy_write_relfenced
+      lc1_src gl1_src
+      lc1_tgt gl1_tgt
+      loc to ord_src ord_tgt
+      (STEP_TGT: Local.racy_write_step lc1_tgt gl1_tgt loc to ord_tgt)
+      (LOCAL1: sim_local lc1_src (local_relfenced lc1_tgt))
+      (GLOBAL1: sim_global gl1_src gl1_tgt)
+      (ORD: Ordering.le ord_src ord_tgt):
+  <<STEP_SRC: Local.racy_write_step lc1_src gl1_src loc to ord_src>>.
+Proof.
+  inv STEP_TGT.
+  exploit sim_local_is_racy_relfenced; eauto.
+Qed.
+
+Lemma sim_local_racy_update_relfenced
+      lc1_src gl1_src
+      lc1_tgt gl1_tgt
+      loc to ordr_src ordw_src ordr_tgt ordw_tgt
+      (STEP_TGT: Local.racy_update_step lc1_tgt gl1_tgt loc to ordr_tgt ordw_tgt)
+      (LOCAL1: sim_local lc1_src (local_relfenced lc1_tgt))
+      (GLOBAL1: sim_global gl1_src gl1_tgt)
+      (ORDR: Ordering.le ordr_src ordr_tgt)
+      (ORDW: Ordering.le ordw_src ordw_tgt):
+  <<STEP_SRC: Local.racy_update_step lc1_src gl1_src loc to ordr_src ordw_src>>.
+Proof.
+  inv STEP_TGT; eauto.
+  exploit sim_local_is_racy_relfenced; eauto.
+Qed.
+
+Lemma sim_local_fence_src_relfenced
+      lc1_src gl1_src
+      lc1_tgt gl1_tgt
+      (LOCAL1: sim_local lc1_src (local_relfenced lc1_tgt))
+      (GLOBAL1: sim_global gl1_src gl1_tgt):
+  exists lc2_src gl2_src,
+    <<STEP_SRC: Local.fence_step lc1_src gl1_src Ordering.plain Ordering.acqrel lc2_src gl2_src>> /\
+    <<LOCAL2: sim_local lc2_src (local_relfenced lc1_tgt)>> /\
+    <<GLOBAL2: sim_global gl2_src gl1_tgt>>.
+Proof.
+  inv LOCAL1. inv TVIEW. ss.
+  esplits.
+  - econs; eauto. i. ss.
+  - econs; eauto. econs; ss; eauto.
+    repeat (condtac; aggrtac).
+  - inv GLOBAL1. ss.
+Qed.
+
+Lemma sim_local_fence_tgt_relfenced
+      lc1_src gl1_src
+      lc1_tgt gl1_tgt
+      lc2_tgt gl2_tgt
+      (STEP_TGT: Local.fence_step lc1_tgt gl1_tgt Ordering.plain Ordering.acqrel lc2_tgt gl2_tgt)
+      (LOCAL1: sim_local lc1_src (local_relfenced lc1_tgt))
+      (GLOBAL1: sim_global gl1_src gl1_tgt)
+      (LC_WF1_SRC: Local.wf lc1_src gl1_src)
+      (LC_WF1_TGT: Local.wf lc1_tgt gl1_tgt):
+  <<LOCAL2: sim_local lc1_src lc2_tgt>> /\
+  <<GLOBAL2: sim_global gl1_src gl2_tgt>>.
+Proof.
+  inv LOCAL1. inv TVIEW. inv STEP_TGT. splits.
+  - econs; ss.
+    unfold TView.read_fence_tview. condtac; ss.
+    unfold TView.write_fence_tview. econs; repeat (condtac; aggrtac).
+  - inv GLOBAL1. ss.
+Qed.
+
+
+Variant sim_release_fenceF: forall R
+                              (st_src:itree MemE.t (unit * R)%type) (lc_src:Local.t) (gl1_src:Global.t)
+                              (st_tgt:itree MemE.t (unit * R)%type) (lc_tgt:Local.t) (gl1_tgt:Global.t), Prop :=
 | sim_relese_fenceF_intro
-    R (v: R) pview
-    lc1_src sc1_src mem1_src
-    lc1_tgt sc1_tgt mem1_tgt
-    (LOCALF: sim_local pview lc1_src (local_relfenced lc1_tgt)):
+    R (v: R)
+    lc1_src gl1_src
+    lc1_tgt gl1_tgt
+    (LOCALF: sim_local lc1_src (local_relfenced lc1_tgt)):
     sim_release_fenceF
-      (Ret (tt, v)) lc1_src sc1_src mem1_src
-      (Vis (MemE.fence Ordering.plain Ordering.acqrel) (fun r => Ret (r, v))) lc1_tgt sc1_tgt mem1_tgt
+      (Ret (tt, v)) lc1_src gl1_src
+      (Vis (MemE.fence Ordering.plain Ordering.acqrel) (fun r => Ret (r, v))) lc1_tgt gl1_tgt
 .
 
 Lemma sim_release_fenceF_step
       R
-      st1_src lc1_src sc0_src mem0_src
-      st1_tgt lc1_tgt sc0_tgt mem0_tgt
-      (SIM: sim_release_fenceF st1_src lc1_src sc0_src mem0_src
-                               st1_tgt lc1_tgt sc0_tgt mem0_tgt):
-  forall sc1_src sc1_tgt
-    mem1_src mem1_tgt
-    (SC: TimeMap.le sc1_src sc1_tgt)
-    (MEMORY: sim_memory mem1_src mem1_tgt)
-    (SC_FUTURE_SRC: TimeMap.le sc0_src sc1_src)
-    (SC_FUTURE_TGT: TimeMap.le sc0_tgt sc1_tgt)
-    (MEM_FUTURE_SRC: Memory.future_weak mem0_src mem1_src)
-    (MEM_FUTURE_TGT: Memory.future_weak mem0_tgt mem1_tgt)
-    (WF_SRC: Local.wf lc1_src mem1_src)
-    (WF_TGT: Local.wf lc1_tgt mem1_tgt)
-    (SC_SRC: Memory.closed_timemap sc1_src mem1_src)
-    (SC_TGT: Memory.closed_timemap sc1_tgt mem1_tgt)
-    (MEM_SRC: Memory.closed mem1_src)
-    (MEM_TGT: Memory.closed mem1_tgt),
+      st1_src lc1_src gl0_src
+      st1_tgt lc1_tgt gl0_tgt
+      (SIM: sim_release_fenceF st1_src lc1_src gl0_src
+                               st1_tgt lc1_tgt gl0_tgt):
+  forall gl1_src gl1_tgt
+    (GLOBAL: sim_global gl1_src gl1_tgt)
+    (LC_WF_SRC: Local.wf lc1_src gl1_src)
+    (LC_WF_TGT: Local.wf lc1_tgt gl1_tgt)
+    (GL_WF_SRC: Global.wf gl1_src)
+    (GL_WF_TGT: Global.wf gl1_tgt),
     _sim_thread_step (lang (unit * R)%type) (lang (unit * R)%type)
-                     ((@sim_thread (lang (unit * R)%type) (lang (unit * R)%type) (sim_terminal eq)) \8/ @sim_release_fenceF R)
-                     st1_src lc1_src sc1_src mem1_src
-                     st1_tgt lc1_tgt sc1_tgt mem1_tgt.
+                     ((@sim_thread (lang (unit * R)%type) (lang (unit * R)%type) (sim_terminal eq)) \6/ @sim_release_fenceF R)
+                     st1_src lc1_src gl1_src
+                     st1_tgt lc1_tgt gl1_tgt.
 Proof.
   destruct SIM; ii. right.
-  inv STEP_TGT; [inv STEP|dependent destruction STEP; inv LOCAL; ss; dependent destruction STATE]; ss.
-  - (* promise *)
-    exploit sim_local_promise_relfenced; eauto. i. des.
+  inv STEP_TGT; ss.
+  { (* internal *)
+    exploit sim_local_internal_relfenced; eauto. i. des.
     esplits.
+    + inv LOCAL; ss.
+    + refl.
+    + econs 2. econs 1. eauto.
     + ss.
-    + eauto.
-    + econs 2. econs 1. econs; eauto.
-    + auto.
-    + auto.
-    + auto.
+    + ss.
     + right. econs 1; eauto.
-  - (* fence *)
-    exploit sim_local_fence_tgt_relfenced; try exact SC; eauto. i. des.
-    esplits.
-    + ss.
-    + eauto.
-    + econs 1.
-    + auto.
-    + auto.
-    + auto.
-    + left. eapply paco11_mon; [apply sim_itree_ret|]; ss.
+  }
+  inv LOCAL; ss; dependent destruction LOCALF; dependent destruction STATE.
+  (* fence *)
+  exploit sim_local_fence_tgt_relfenced; try exact GLOBAL; eauto. i. des.
+  esplits.
+  + ss.
+  + refl.
+  + econs 1.
+  + ss.
+  + ss.
+  + left. eapply paco9_mon; [apply sim_itree_ret|]; ss.
 Qed.
 
 Lemma sim_release_fenceF_sim_thread R:
-  @sim_release_fenceF R <8= (@sim_thread (lang (unit * R)%type) (lang (unit * R)%type) (sim_terminal eq)).
+  @sim_release_fenceF R <6= (@sim_thread (lang (unit * R)%type) (lang (unit * R)%type) (sim_terminal eq)).
 Proof.
   pcofix CIH. i. pfold. ii. ss. splits; ss; ii.
   - right. inv TERMINAL_TGT. inv PR; ss.
   - right. inv PR.
     esplits; eauto.
-    eapply sim_local_memory_bot; eauto.
-  - exploit sim_release_fenceF_step; try apply PR; try apply SC; eauto. i. des; eauto.
+    inv LOCALF. ss. congr.
+  - exploit sim_release_fenceF_step; try apply PR; try apply GLOBAL; eauto. i. des; eauto.
     + right. esplits; eauto.
-      left. eapply paco11_mon; eauto. ss.
+      left. eapply paco9_mon; eauto. ss.
     + right. esplits; eauto.
 Qed.
 
@@ -139,144 +457,115 @@ Lemma reorder_release_fenceF_sim_itree R
 Proof.
   pcofix CIH. ii. subst. pfold. ii. splits; ii.
   { inv TERMINAL_TGT. eapply f_equal with (f:=observe) in H; ss. }
-  { right. esplits; eauto.
-    inv LOCAL. apply SimPromises.sem_bot_inv in PROMISES; auto. rewrite PROMISES. auto.
-  }
+  { right. esplits; eauto. inv LOCAL. congr. }
   inv STEP_TGT.
-  { (* promise *)
+  { (* internal *)
     right.
-    inv STEP.
-    exploit sim_local_promise_bot; eauto. i. des.
-    esplits; try apply SC; eauto; ss.
-    econs 2. econs 1; eauto. econs; eauto.
+    exploit sim_local_internal; eauto. i. des.
+    esplits; try apply GL2; eauto; ss.
+    inv LOCAL0; ss.
   }
-  exploit sim_local_intro_relfenced; eauto. i. des.
-  exploit sim_local_nonsynch_src; try exact SC_SRC; eauto using local_relfenced_wf. i. des.
-  instantiate (3:=lang (unit * R)) in STEP_SRC.
-  instantiate (2:=Vis (MemE.fence Ordering.plain Ordering.acqrel)
-                      (fun r0 => Vis i1 (fun r => Ret (r0, r)))) in STEP_SRC.
-  exploit Thread.rtc_tau_step_future; eauto. s. i. des.
+  exploit sim_local_relfenced; eauto. i.
   exploit sim_local_fence_src_relfenced; eauto. i. des.
   exploit Local.fence_step_future; eauto. i. des.
-  inv STEP. inv LOCAL1; ss; dependent destruction STATE; inv REORDER.
+  inv LOCAL0; ss; dependent destruction REORDER; dependent destruction STATE.
   - (* load *)
     right.
     exploit sim_local_read_relfenced; eauto; try refl. i. des.
     esplits.
     + ss.
-    + etrans; [eauto|]. econs 2; [|refl]. econs.
-      * econs. econs 2. econs; [|econs 5]; eauto. econs. econs.
+    + econs 2; [|refl]. econs.
+      * econs 2; [|econs 5]; eauto. econs. refl.
       * ss.
-    + econs 2. econs 2. econs; [|econs 2]; eauto. econs. econs.
-    + auto.
-    + etrans; eauto.
-    + auto.
-    + left. eapply paco11_mon; [apply sim_release_fenceF_sim_thread|]; ss.
-      econs. eauto.
+    + econs 2. econs 2; [|econs 2]; eauto. econs. refl.
+    + ss.
+    + ss.
+    + left. eapply paco9_mon; [apply sim_release_fenceF_sim_thread|]; ss.
   - (* update-load *)
     right.
     guardH ORDW2.
     exploit sim_local_read_relfenced; eauto; try refl. i. des.
     esplits.
     + ss.
-    + etrans; [eauto|]. econs 2; [|refl]. econs.
-      * econs. econs 2. econs; [|econs 5]; eauto. econs. econs.
+    + econs 2; [|refl]. econs.
+      * econs 2; [|econs 5]; eauto. econs. refl.
       * ss.
-    + econs 2. econs 2. econs; [|econs 2]; eauto. econs; eauto.
-    + auto.
-    + etrans; eauto.
-    + auto.
-    + left. eapply paco11_mon; [apply sim_release_fenceF_sim_thread|]; ss.
-      econs. eauto.
+    + econs 2. econs 2; [|econs 2]; eauto. econs; eauto.
+    + ss.
+    + ss.
+    + left. eapply paco9_mon; [apply sim_release_fenceF_sim_thread|]; ss.
   - (* write *)
     right.
     guardH ORD21.
-    hexploit sim_local_write_relfenced; try exact SC;
+    hexploit sim_local_write_relfenced; try exact GLOBAL2;
       try match goal with
           | [|- is_true (Ordering.le _ _)] => refl
           end; eauto; (try by econs). i. des.
     esplits.
     + ss.
-    + etrans; [eauto|]. econs 2; [|refl]. econs.
-      * econs. econs 2. econs; [|econs 5]; eauto. econs. econs.
+    + econs 2; [|refl]. econs.
+      * econs 2; [|econs 5]; eauto. econs. refl.
       * ss.
-    + econs 2. econs 2. econs; [|econs 3]; eauto. econs. econs.
-      replace sc2_src with sc1_src; eauto. apply TimeMap.antisym; ss.
-    + auto.
-    + auto.
-    + auto.
-    + left. eapply paco11_mon; [apply sim_release_fenceF_sim_thread|]; ss.
-      econs. eauto.
+    + econs 2. econs 2; [|econs 3]; eauto. econs. refl.
+    + ss.
+    + ss.
+    + left. eapply paco9_mon; [apply sim_release_fenceF_sim_thread|]; ss.
   - (* update *)
     right.
     guardH ORDW2.
     exploit Local.read_step_future; eauto. i. des.
     exploit sim_local_read_relfenced; eauto; try refl. i. des.
     exploit Local.read_step_future; eauto. i. des.
-    hexploit sim_local_write_relfenced; try exact SC;
+    hexploit sim_local_write_relfenced; try exact GLOBAL2;
       try match goal with
           | [|- is_true (Ordering.le _ _)] => refl
           end; eauto; (try by econs). i. des.
     esplits.
     + ss.
-    + etrans; [eauto|]. econs 2; [|refl]. econs.
-      * econs. econs 2. econs; [|econs 5]; eauto. econs. econs.
+    + econs 2; [|refl]. econs.
+      * econs 2; [|econs 5]; eauto. econs. refl.
       * ss.
-    + econs 2. econs 2. econs; [|econs 4]; eauto.
-      * econs; eauto.
-      * replace sc2_src with sc1_src; eauto. apply TimeMap.antisym; ss.
-    + auto.
-    + auto.
-    + auto.
-    + left. eapply paco11_mon; [apply sim_release_fenceF_sim_thread|]; ss.
-      econs. eauto.
+    + econs 2. econs 2; [|econs 4]; eauto. econs; eauto.
+    + ss.
+    + ss.
+    + left. eapply paco9_mon; [apply sim_release_fenceF_sim_thread|]; ss.
   - (* fence *)
     right.
-    exploit sim_local_fence_relfenced; try exact SC; eauto; try refl. i. des.
+    exploit sim_local_fence_relfenced; try exact GLOBAL2; eauto; try refl. i. des.
     esplits.
     + ss.
-    + etrans; [eauto|]. econs 2; [|refl]. econs.
-      * econs. econs 2. econs; [|econs 5]; eauto. econs. econs.
+    + econs 2; [|refl]. econs.
+      * econs 2; [|econs 5]; eauto. econs. refl.
       * ss.
-    + econs 2. econs 2. econs; [|econs 5]; eauto.
-      * econs. econs.
-      * replace sc2_src with sc1_src; eauto. apply TimeMap.antisym; ss.
-    + auto.
-    + auto.
-    + auto.
-    + left. eapply paco11_mon; [apply sim_release_fenceF_sim_thread|]; ss.
-      econs. eauto.
-  - (* na write *)
-    inv LOCAL3. destruct ord; ss.
+    + econs 2. econs 2; [|econs 5]; eauto. econs. refl.
+    + ss.
+    + ss.
+    + left. eapply paco9_mon; [apply sim_release_fenceF_sim_thread|]; ss.
   - (* racy read *)
     right.
     exploit sim_local_racy_read_relfenced; eauto; try refl. i. des.
     esplits.
     + ss.
-    + etrans; [eauto|]. econs 2; [|refl]. econs.
-      * econs. econs 2. econs; [|econs 5]; eauto. econs. econs.
+    + econs 2; [|refl]. econs.
+      * econs 2; [|econs 5]; eauto. econs. refl.
       * ss.
-    + econs 2. econs 2. econs; [|econs 9]; eauto. econs. econs.
-    + auto.
-    + etrans; eauto.
-    + auto.
-    + left. eapply paco11_mon; [apply sim_release_fenceF_sim_thread|]; ss.
-      econs. eauto.
+    + econs 2. econs 2; [|econs 8]; eauto. econs. refl.
+    + ss.
+    + ss.
+    + left. eapply paco9_mon; [apply sim_release_fenceF_sim_thread|]; ss.
   - (* racy update-load *)
     right.
     guardH ORDW2.
     exploit sim_local_racy_read_relfenced; eauto; try refl. i. des.
     esplits.
     + ss.
-    + etrans; [eauto|]. econs 2; [|refl]. econs.
-      * econs. econs 2. econs; [|econs 5]; eauto. econs. econs.
+    + econs 2; [|refl]. econs.
+      * econs 2; [|econs 5]; eauto. econs. refl.
       * ss.
-    + econs 2. econs 2. econs; [|econs 9]; eauto. econs; eauto.
-    + auto.
-    + etrans; eauto.
-    + auto.
-    + left. eapply paco11_mon; [apply sim_release_fenceF_sim_thread|]; ss.
-      econs. eauto.
+    + econs 2. econs 2; [|econs 8]; eauto. econs; eauto.
+    + ss.
+    + ss.
+    + left. eapply paco9_mon; [apply sim_release_fenceF_sim_thread|]; ss.
   - (* racy write *)
     left.
     guardH ORD21.
@@ -284,11 +573,11 @@ Proof.
       try match goal with
           | [|- is_true (Ordering.le _ _)] => refl
           end; eauto. i. des.
-    unfold Thread.steps_failure. esplits.
-    + etrans; [eauto|]. econs 2; [|refl]. econs.
-      * econs. econs 2. econs; [|econs 5]; eauto. econs. econs.
+    econs.
+    + econs 2; [|refl]. econs.
+      * econs 2; [|econs 5]; eauto. econs. refl.
       * ss.
-    + econs 2. econs; [|econs 10]; eauto. econs. econs.
+    + econs 2; [|econs 9]; eauto. econs. refl.
     + ss.
   - (* racy update *)
     left.
@@ -297,10 +586,10 @@ Proof.
       try match goal with
           | [|- is_true (Ordering.le _ _)] => refl
           end; eauto. i. des.
-    unfold Thread.steps_failure. esplits.
-    + etrans; [eauto|]. econs 2; [|refl]. econs.
-      * econs. econs 2. econs; [|econs 5]; eauto. econs. econs.
+    econs.
+    + econs 2; [|refl]. econs.
+      * econs 2; [|econs 5]; eauto. econs. refl.
       * ss.
-    + econs 2. econs; [|econs 11]; eauto. econs; eauto.
+    + econs 2; [|econs 10]; eauto. econs; eauto.
     + ss.
 Qed.
